chore(Keller): split out smaller files, clean up definitions a bit

Experiments/Keller/G8_Clique.lean
@@ -1,8 +1,44 @@
 import Experiments.Keller.KellerGraph
 
+namespace Keller
+
+structure KCliqueData (n s : Nat) where
+  vertices : Vector (Vector (Fin s) n) (2^n)
+deriving Repr
+
+instance : ToString (KCliqueData n s) where
+  toString := fun kc => toString <| kc.vertices.toArray.map (·.toArray)
+
+def KCliqueData.get (i : BitVec n) (kc : KCliqueData n s): KVertex n s :=
+  { bv := i, colors := kc.vertices[i.toFin] }
+
+def KCliqueData.getEmbedding (kc : KCliqueData n s) : BitVec n ↪ KVertex n s :=
+  ⟨kc.get, by intro a; simp [get]⟩
+
+def KCliqueData.checkAll (kc : KCliqueData n s) : Bool :=
+  decide (∀ i i' : Fin (2^n), i < i' → KAdj (kc.get i) (kc.get i'))
+
+theorem KCliqueData.checkAll_implies_not_conjecture (kc : KCliqueData n s)
+  : kc.checkAll = true → ¬ conjectureIn n := by
+  simp [checkAll, conjectureIn]
+  intro h
+  use s, (Finset.univ |>.map kc.getEmbedding)
+  constructor
+  · intro x hx y hy hne; simp at hx hy
+    rcases hx with ⟨⟨xi⟩,rfl⟩
+    rcases hy with ⟨⟨yi⟩,rfl⟩
+    simp at hne
+    wlog hlt : xi < yi generalizing xi yi
+    · apply SimpleGraph.adj_symm
+      apply this; exact Ne.symm hne; omega
+    specialize h xi yi hlt
+    convert h using 1
+      <;> simp [getEmbedding, BitVec.ofNat]
+  · simp
+
 set_option maxRecDepth 800 in
-def G8_clique: KellerCliqueData 8 2 :=
-  KellerCliqueData.mk <| Vector.mk #[
+def G8_clique: KCliqueData 8 2 :=
+  KCliqueData.mk <| Vector.mk #[
   v 0 0 0 0 0 0 0 0, v 0 0 1 0 0 0 0 0, v 1 0 1 0 1 1 0 1, v 1 0 1 0 1 0 1 1,
   v 0 0 0 1 1 0 1 1, v 0 1 1 1 1 1 0 1, v 0 0 1 0 0 0 0 0, v 0 1 1 0 0 0 0 0,
   v 0 1 0 0 0 0 0 0, v 0 1 1 0 0 0 0 0, v 1 1 0 0 1 0 1 1, v 1 1 0 0 1 1 0 1,
@@ -71,4 +107,7 @@ def G8_clique: KellerCliqueData 8 2 :=
 where v (a b c d e f g h) : Vector (Fin 2) 8 :=
   Vector.mk #[a,b,c,d,e,f,g,h] (by simp)
 
-example : checkAll G8_clique = true := by native_decide
+theorem not_conjectureIn_8 : ¬ conjectureIn 8 := by
+  apply G8_clique.checkAll_implies_not_conjecture
+  native_decide
+
