Experiments/Keller/Autos.lean
@@ -1,0 +1,176 @@
+import Experiments.Keller.KellerGraph
+
+namespace Keller
+
+def KAuto (n s) := SimpleGraph.Iso (KGraph n s) (KGraph n s)
+
+def KClique.map (a : KAuto n s) (k : KClique n s) : KClique n s :=
+  ⟨(k.val.map a.toEmbedding.toEmbedding), by
+  have ⟨vs,{card_eq, isClique}⟩ := k
+  simp only [KClique, SimpleGraph.isNClique_iff,
+    Finset.card_map, card_eq, and_true]
+  clear card_eq
+  generalize hvs' : vs.map _ = vs'
+  simp [Finset.ext_iff] at hvs'
+  intro v₁ hv₁ v₂ hv₂ hne
+  simp [← hvs'] at hv₁ hv₂; clear hvs'
+  rcases hv₁ with ⟨v₁,hv₁,rfl⟩; rcases hv₂ with ⟨v₂,hv₂,rfl⟩
+  apply a.map_adj_iff.mpr
+  simp [SimpleGraph.isClique_iff]
+  replace hne : v₁ ≠ v₂ := fun h => hne (congrArg a.toFun h)
+  apply isClique ?_ ?_ hne <;> simp [hv₁, hv₂]
+  ⟩
+
+
+namespace KVertex
+
+def flip (mask : BitVec n) (v : KVertex n s) : KVertex n s :=
+  { bv := v.bv ^^^ mask, colors := v.colors }
+
+theorem bv_flip (mask) {v : KVertex n s} : (flip mask v).bv = v.bv ^^^ mask := rfl
+@[simp] theorem bv_colors (mask) {v : KVertex n s} : (flip mask v).colors = v.colors := rfl
+
+@[simp] theorem flip_flip (mask : BitVec n) {v : KVertex n s} : (v.flip mask).flip mask = v := by
+  simp [flip, BitVec.xor_assoc]
+
+
+def permute (f : Fin n → Fin s → Fin s) (v : KVertex n s) : KVertex n s :=
+  { bv := v.bv, colors := Vector.ofFn (fun j => (f j) v.colors[j]) }
+
+@[simp] theorem bv_permute (f) {v : KVertex n s} : (permute f v).bv = v.bv := rfl
+
+theorem colors_permute (f) (v : KVertex n s) {j h} :
+    (permute f v).colors[j]'h = (f ⟨j,h⟩) v.colors[j] := by
+  simp [permute]
+
+
+theorem permute_permute (f₁ f₂ : Fin n → Fin s → Fin s) {v} :
+    permute f₁ (permute f₂ v) = permute (fun j => f₁ j ∘ f₂ j) v := by
+  simp [permute]
+
+@[simp] theorem permute_id {v : KVertex n s} : permute (fun _ => id) v = v := by
+  simp [permute]
+  congr
+  ext i hi
+  simp
+
+
+def reorder (f : Fin n → Fin n) (v : KVertex n s) : KVertex n s :=
+  ⟨ BitVec.ofFn (v.bv[f ·])
+  , Vector.ofFn (v.colors[f ·])⟩
+
+theorem bv_reorder (f : Fin n → Fin n) (v : KVertex n s) {j hj} :
+    (v.reorder f).bv[j]'hj = v.bv[f ⟨j,hj⟩] := by
+  simp [reorder]
+
+theorem colors_reorder (f : Fin n → Fin n) (v : KVertex n s) {j hj} :
+    (v.reorder f).colors[j]'hj = v.colors[f ⟨j,hj⟩] := by
+  simp [reorder]
+
+theorem reorder_comp (f₁ f₂ : Fin n → Fin n) (v : KVertex n s)
+    : reorder f₁ (reorder f₂ v) = reorder (f₂ ∘ f₁) v := by
+  simp [reorder]
+
+@[simp] theorem reorder_id (v : KVertex n s) : reorder id v = v := by
+  ext <;> simp [reorder]
+
+end KVertex
+
+
+namespace KAuto
+
+def id : KAuto n s := RelIso.refl _
+
+def flip (mask : BitVec n) : KAuto n s :=
+  RelIso.mk ({
+    toFun := KVertex.flip mask
+    invFun := KVertex.flip mask
+    left_inv  := by intro; simp
+    right_inv := by intro; simp
+  }) (by
+    simp [KAdj, KVertex.bv_flip]
+  )
+
+@[simp] theorem toFun_flip {x : KVertex _ _ } :
+  DFunLike.coe (F := KAdj ≃r KAdj) (α := KVertex n s) (β := fun _ => KVertex n s)
+    (flip (n := n) (s := s) mask) x = KVertex.flip mask x := rfl
+
+def permute (f : Fin n → Fin s ≃ Fin s) : KAuto n s :=
+  RelIso.mk ({
+    toFun := KVertex.permute (fun j => f j)
+    invFun := KVertex.permute (fun j => (f j).symm)
+    left_inv  := by intro; simp [KVertex.permute_permute]
+    right_inv := by intro; simp [KVertex.permute_permute]
+  }) (by
+    intro v₁ v₂
+    simp [KAdj, KVertex.colors_permute])
+
+@[simp] theorem toFun_permute {x : KVertex _ _ } :
+  DFunLike.coe (F := KAdj ≃r KAdj) (α := KVertex n s) (β := fun _ => KVertex n s)
+    (permute (n := n) (s := s) f) x = KVertex.permute (fun j => f j) x := rfl
+
+def reorder (f : Fin n ≃ Fin n) : KAuto n s :=
+  RelIso.mk {
+    toFun := KVertex.reorder f
+    invFun := KVertex.reorder f.invFun
+    left_inv := by intro; simp [KVertex.reorder_comp]
+    right_inv := by intro; simp [KVertex.reorder_comp]
+  } (by
+    intro a b
+    simp [KAdj, KVertex.reorder]
+    constructor
+    · rintro ⟨j₁,hbv₁,hc1,j₂,hne,h⟩
+      use f j₁, hbv₁, hc1, f j₂
+      rw [EmbeddingLike.apply_eq_iff_eq]
+      simp [hne, h]
+    · rintro ⟨j₁,hbv₁,hc1,j₂,hne,h⟩
+      use f.symm j₁; simp
+      use hbv₁, hc1, f.symm j₂
+      rw [EmbeddingLike.apply_eq_iff_eq]
+      simp [hne, h]
+  )
+
+@[simp] theorem toFun_reorder {x : KVertex _ _ } :
+  DFunLike.coe (F := KAdj ≃r KAdj) (α := KVertex n s) (β := fun _ => KVertex n s)
+    (reorder (n := n) (s := s) f) x = KVertex.reorder (fun j => f j) x := rfl
+
+def swap [DecidableEq α] (L : List (α × α)) : α ≃ α :=
+  match L with
+  | [] => Equiv.refl _
+  | (a,b) :: tail => (swap tail).insert a b
+
+@[simp] theorem swap_nil [DecidableEq α] : swap (α := α) [] i = i := rfl
+
+@[simp] theorem swap_cons_of_eq_left [DecidableEq α] :
+    swap (α := α) ((i,o) :: tail) i = o := by
+  simp [swap]
+
+@[simp] theorem swap_cons_of_eq_right [DecidableEq α]
+      (htail : swap tail i' = o) :
+    swap (α := α) ((i,o) :: tail) i' = swap tail i := by
+  simp [swap, htail]; rw [Equiv.insert_right]; exact htail
+
+@[simp] theorem swap_cons_of_ne [DecidableEq α]
+      (hhead : i' ≠ i) (htail : swap tail i' ≠ o) :
+    swap (α := α) ((i,o) :: tail) i' = swap tail i' := by
+  simp [swap, htail]; rw [Equiv.insert_unchanged] <;> assumption
+
+theorem swap_eq_of_mem [DecidableEq α] (L : List (α × α))
+    (is_distinct : L.Pairwise (·.1 ≠ ·.1)) (os_distinct : L.Pairwise (·.2 ≠ ·.2))
+    (pair_mem : (i,o) ∈ L) :
+    swap L i = o := by
+  induction L generalizing i o with
+  | nil => simp at pair_mem
+  | cons hd tl ih =>
+    simp at pair_mem
+    rcases pair_mem with (rfl|pair_mem)
+    case inl => simp
+    case inr =>
+    specialize ih is_distinct.tail os_distinct.tail pair_mem
+    replace is_distinct := Ne.symm <| List.rel_of_pairwise_cons is_distinct pair_mem
+    replace os_distinct := Ne.symm <| List.rel_of_pairwise_cons os_distinct pair_mem
+    clear pair_mem
+    rcases hd with ⟨x,y⟩; dsimp at is_distinct os_distinct ⊢
+    simp [swap]; rw [← ih] at os_distinct ⊢
+    apply Equiv.insert_unchanged <;> assumption
+
