Experiments/Keller/SymmBreak.lean
@@ -1,0 +1,181 @@
+import Experiments.Keller.Autos
+
+namespace Keller
+
+structure SB0 (n s) where
+  kclique : KClique n s
+
+structure SB1 (n s) extends SB0 (n+2) (s+1) where
+  c0 : kclique.get 0 = ⟨Array.mkArray (n+2) 0, by simp⟩
+  c1 : kclique.get 1 = ⟨#[0,1] ++ Array.mkArray n 0, by simp; omega⟩
+
+theorem SB0.pick_pair {n s} (x : SB0 (n+2) (s+1)) (h : conjectureIn (n+1))
+  : ∃ (i₁ i₂ : BitVec (n+2)) (j₁ j₂ : Fin (n+2)), j₁ ≠ j₂ ∧ ∀ j (h : j < n+2),
+      (j ≠ j₁ ↔ i₁[j] = i₂[j]) ∧
+      (j ≠ j₂ ↔ (x.kclique.get i₁)[j] = (x.kclique.get i₂)[j])
+  := by
+  let K_0 : Finset (KVertex (n+1) (s+1)) := (Finset.univ (α := BitVec (n+1)))
+    |>.map ⟨fun i =>
+        let i' := i.cons false
+        let v := x.kclique.get i'
+        ⟨i, v.take (n+1) |>.cast (by omega)⟩
+      , by
+        intro x1 x2 heq
+        simp at heq; exact heq.1⟩
+  have K_0_card : K_0.card = (2^(n+1)) := by simp [K_0]
+  have K_0_not_clique : ¬ _ := (h (s+1)).false ∘ Subtype.mk K_0
+  -- find the vertices in K_0 which are the not adjacent
+  simp [KClique, SimpleGraph.isNClique_iff, K_0_card,
+      SimpleGraph.isClique_iff, Set.Pairwise] at K_0_not_clique
+  clear K_0_card h
+  rcases K_0_not_clique with ⟨⟨i₁,c₁⟩, hv₁, ⟨i₂,c₂⟩, hv₂, hne, hnotadj⟩
+  simp [K_0] at hv₁ hv₂; clear K_0
+  -- the indices in smaller graph must be diff
+  have i_diff : i₁ ≠ i₂ := by
+    intro contra; subst hv₁ hv₂; simp [contra] at hne
+  clear hne
+  -- name the corresponding colors in bigger graph
+  generalize hk₁ : KClique.get _ _ = k₁ at hv₁
+  generalize hk₂ : KClique.get _ _ = k₂ at hv₂
+  subst hv₁ hv₂
+  -- the corresponding vertices are adjacent in big graph
+  have : KAdj ⟨i₁.cons false, k₁⟩ ⟨i₂.cons false,k₂⟩ := by
+    subst hk₁ hk₂
+    apply x.kclique.isClique
+    iterate 2 (apply KClique.get_mem)
+    simp [i_diff]
+  simp [KAdj] at this hnotadj
+  rcases this with ⟨⟨j₁,hj₁⟩,is_have_diff,ks_same,⟨j₂,hj₂⟩,js_diff,h⟩
+  simp_all
+  -- the i's are different at index j₁
+  have : j₁ ≠ n+1 := by intro contra; simp [BitVec.getElem_cons, contra] at is_have_diff
+  simp [BitVec.getElem_cons, this] at is_have_diff
+  replace hj₁ : j₁ < n+1 := by omega
+  clear this
+  specialize hnotadj ⟨j₁, hj₁⟩ is_have_diff ks_same
+  -- j₂ must be n+1
+  by_cases this : j₂ = n+1
+  case neg =>
+    exfalso
+    replace hj₂ : j₂ < n+1 := by omega
+    specialize hnotadj ⟨j₂,hj₂⟩
+    simp [js_diff] at hnotadj
+    simp [BitVec.getElem_cons, Nat.ne_of_lt hj₂, hnotadj.2] at h
+    apply h hnotadj.1
+  subst this
+  simp [BitVec.getElem_cons] at h
+  -- now we fill the goal
+  use (i₁.cons false), (i₂.cons false), ⟨j₁,‹_›⟩, ⟨n+1, by omega⟩
+  simp [hk₁, hk₂, js_diff]
+  rintro j -
+  by_cases eq_j1 : j = j₁
+  · simp_all [BitVec.getElem_cons]
+  · by_cases eq_last : j = n+1
+    · simp_all [BitVec.getElem_cons]
+    · specialize hnotadj ⟨j, by omega⟩ (by simp; exact Ne.symm eq_j1)
+      simp_all [BitVec.getElem_cons]; exact hnotadj.1
+
+def SB0.reorder (j₁ j₂ : Fin (n+2)) := KAuto.swap [(0,j₁), (1,j₂)]
+
+@[simp] theorem SB0.reorder_0 (j1 j2 : Fin (n+2)) : reorder j1 j2 0 = j1 := by
+  simp [reorder]
+@[simp] theorem SB0.reorder_eq_j1 (j1 j2 : Fin (n+2)) : reorder j1 j2 j = j1 ↔ j = 0 := by
+  conv => lhs; rhs; rw [← SB0.reorder_0 j1 j2]
+  rw [Equiv.apply_eq_iff_eq]
+@[simp] theorem SB0.reorder_1 (j1 j2 : Fin (n+2)) (h : j1 ≠ j2) : reorder j1 j2 1 = j2 := by
+  simp [reorder]; rw [KAuto.swap_eq_of_mem] <;> simp [h]
+@[simp] theorem SB0.reorder_eq_j2 (j1 j2 : Fin (n+2)) (h : j1 ≠ j2) : reorder j1 j2 j = j2 ↔ j = 1 := by
+  conv => lhs; rhs; rw [← SB0.reorder_1 j1 j2 h]
+  rw [Equiv.apply_eq_iff_eq]
+
+/-- The automorphism which moves v₁ to ⟨0,[0*]⟩ and v₂ to ⟨1,[0,1,0*]⟩ -/
+def SB0.auto {n s} (v₁ v₂ : KVertex (n+2) (s+2)) : KAuto (n+2) (s+2) :=
+  (KAuto.flip v₁.bv)
+  |>.trans (KAuto.permute fun j =>
+    if j = 1 then
+      KAuto.swap [(v₁.colors[j], 0), (v₂.colors[j], 1)]
+    else
+      KAuto.swap [(v₁.colors[j], 0)]
+  )
+
+theorem SB0.auto_v₁ {v₁ v₂ : KVertex (n+2) (s+2)} :
+      (SB0.auto v₁ v₂).toFun v₁ = ⟨0, Vector.mkVector _ 0⟩ := by
+  ext j hj
+  · unfold auto; simp [KVertex.bv_flip]
+  · unfold auto; simp [KVertex.colors_permute, Vector.mkVector]
+    if hj : j = 1 then
+      simp [hj]
+    else
+      simp [← Fin.val_eq_val, hj]
+
+theorem SB0.auto_v₂ {v₁ v₂ : KVertex (n+2) (s+2)}
+      (h : ∀ j (h : j < n+2),
+          (j ≠ 0 ↔ v₁.bv[j] = v₂.bv[j]) ∧
+          (j ≠ 1 ↔ v₁.colors[j] = v₂.colors[j])) :
+      (SB0.auto v₁ v₂).toFun v₂ = ⟨1, ⟨#[0,1] ++ Array.mkArray n 0, by simp; omega⟩⟩ := by
+  ext j hj <;> specialize h j hj
+  · replace h := h.1
+    unfold auto; simp [KVertex.bv_flip]
+    by_cases j = 0 <;> aesop
+  · replace h := h.2
+    unfold auto; simp [KVertex.colors_permute, Vector.mkVector]
+    if hj : j = 1 then
+      simp [hj, Array.getElem_append]
+      simp [hj] at h
+      rw [KAuto.swap_eq_of_mem]
+      case is_distinct => simp [h]
+      case os_distinct => simp
+      case pair_mem => simp; right; rfl
+      rfl
+    else
+      simp [hj] at h
+      simp [← Fin.val_eq_val, hj, h, Array.getElem_append]
+      split
+      · have : j = 0 := by omega
+        simp [this]
+      · rfl
+
+theorem SB0.to_SB1 {n s} (k : SB0 (n+2) (s+2)) (h : conjectureIn (n+1))
+  : Nonempty (SB1 n (s+1)) := by
+  have ⟨ai, bi, j₁, j₂, hne, same_on⟩ := k.pick_pair h
+  -- clean up the context a *bunch*
+  -- TODO(JG): just change pick_pair to be in the form I actually want it in
+  clear h; rcases k with ⟨k⟩
+  generalize a_mem_vs : k.get ai = a_cs at same_on
+  generalize b_mem_vs : k.get bi = b_cs at same_on
+  rw [KClique.get_eq_iff_mem] at a_mem_vs b_mem_vs
+  generalize ha : KVertex.mk ai a_cs = a at a_mem_vs
+  generalize hb : KVertex.mk bi b_cs = b at b_mem_vs
+  simp [KVertex.ext_iff] at ha hb
+  rcases ha with ⟨rfl,rfl⟩; rcases hb with ⟨rfl,rfl⟩
+  -- okay, context is now pretty reasonable
+  -- apply the reordering automorphism to get vs2, k2, a2, b2
+  let k2 := k.map (KAuto.reorder <| SB0.reorder j₁ j₂)
+  let a2 := (KAuto.reorder (reorder j₁ j₂)).toFun a
+  let b2 := (KAuto.reorder (reorder j₁ j₂)).toFun b
+  -- apply the "move to all 0s" automorphism to get vs3, k3
+  let k3 := k2.map (SB0.auto a2 b2)
+
+  -- k3 is the clique we want! just have to prove 0 ↦ 0*, 1 ↦ 0,1,0*
+  refine ⟨{kclique := k3, c0 := ?c0, c1 := ?c1}⟩
+  case c0 =>
+    rw [KClique.get_eq_iff_mem]; simp [k3, KClique.map]
+    use a2
+    constructor
+    · apply Finset.mem_map_of_mem; exact a_mem_vs
+    · apply SB0.auto_v₁
+  case c1 =>
+    rw [KClique.get_eq_iff_mem]; simp [k3, KClique.map]
+    use b2
+    constructor
+    · apply Finset.mem_map_of_mem; exact b_mem_vs
+    · apply SB0.auto_v₂
+      intro j hj
+      simp [a2, b2, KVertex.bv_reorder, KVertex.colors_reorder]
+      constructor
+      · rw [← (same_on _ _).1, not_iff_not, Fin.val_eq_val,
+          SB0.reorder_eq_j1, ← Fin.val_eq_val]
+        rfl
+      · rw [← (same_on _ _).2, not_iff_not, Fin.val_eq_val,
+          SB0.reorder_eq_j2 _ _ hne, ← Fin.val_eq_val]
+        rfl
